Split FLC message types into concrete and assertion

tlc/comp/flc.v
@@ -1,5 +1,7 @@
 From mathcomp.ssreflect
 Require Import ssreflect eqtype ssrbool.
+From tlc.assert
+Require Import node_variable message_variable.
 
 Set Implicit Arguments.
 Unset Strict Implicit.
@@ -10,72 +12,144 @@ Section flc.
   Variable node : eqType.
   Variable message : eqType.
 
-  (* Requests *)
-
+  (* Concrete requests *)
   Inductive req_fl_ : Type :=
   | Send_fl : node -> message -> req_fl_.
 
   (* Equality *)
+  Section req_fl__eq.
 
-  Definition eq_req_fl_ (r r' : req_fl_) : bool :=
-    match r, r' with
-    | Send_fl n m, Send_fl n' m' => [&& n == n' & m == m']
-    end.
+    Definition eq_req_fl_ (r r' : req_fl_) :=
+      match r, r' with
+      | Send_fl n m, Send_fl n' m' => (n == n') && (m == m')
+      end.
 
-  Lemma eq_req_fl_P : Equality.axiom eq_req_fl_.
-  Proof.
-    case => [ n m ];
-    case => [ n' m' ];
-    rewrite /=; try by constructor.
-    - (* Send_fl *)
-      case Hn: (n == n');
-        [move/eqP: Hn => ?; subst n' | constructor];
-        last by case=> ?; subst n'; rewrite eqxx in Hn.
-      case Hm: (m == m');
-        [move/eqP: Hm => ?; subst m' | constructor];
-        last by case=> ?; subst m'; rewrite eqxx in Hm.
-      by constructor.
-  Qed.
+    Lemma eq_req_fl_P : Equality.axiom eq_req_fl_.
+    Proof.
+      case=> [n m]; case=> [n' m'];
+        rewrite /eq_req_fl_ /=; try by constructor.
+      - (* Send_fl *)
+        case Hn: (n == n');
+          [move/eqP: Hn => ?; subst n' | constructor];
+          last by case=> ?; subst n'; rewrite eqxx in Hn.
+        case Hm: (m == m');
+          [move/eqP: Hm => ?; subst m' | constructor];
+          last by case=> ?; subst m'; rewrite eqxx in Hm.
+        by constructor.
+    Qed.
 
-  Canonical req_fl__eqMixin :=
-    Eval hnf in EqMixin eq_req_fl_P.
-  Canonical req_fl__eqType :=
-    Eval hnf in EqType req_fl_ req_fl__eqMixin.
+    Canonical req_fl__eqMixin :=
+      Eval hnf in EqMixin eq_req_fl_P.
+    Canonical req_fl__eqType :=
+      Eval hnf in EqType req_fl_ req_fl__eqMixin.
 
-  Definition req_fl := [eqType of req_fl_].
+    Definition req_fl := [eqType of req_fl_].
 
-  (* Indications *)
+  End req_fl__eq.
 
+  (* Assertion requests *)
+  Inductive req_fl_A_ : Type :=
+  | Send_fl_A : node_variable -> message_variable -> req_fl_A_.
+
+  (* Equality *)
+  Section req_fl_A__eq.
+
+    Definition eq_req_fl_A_ (r r' : req_fl_A_) :=
+      match r, r' with
+      | Send_fl_A n m, Send_fl_A n' m' => (n == n') && (m == m')
+      end.
+
+    Lemma eq_req_fl_A_P : Equality.axiom eq_req_fl_A_.
+    Proof.
+      case=> [n m]; case=> [n' m'];
+        rewrite /eq_req_fl_A_ /=; try by constructor.
+      - (* Send_fl_A *)
+        case Hn: (n == n');
+          [move/eqP: Hn => ?; subst n' | constructor];
+          last by case=> ?; subst n'; rewrite eqxx in Hn.
+        case Hm: (m == m');
+          [move/eqP: Hm => ?; subst m' | constructor];
+          last by case=> ?; subst m'; rewrite eqxx in Hm.
+        by constructor.
+    Qed.
+
+    Canonical req_fl_A__eqMixin :=
+      Eval hnf in EqMixin eq_req_fl_A_P.
+    Canonical req_fl_A__eqType :=
+      Eval hnf in EqType req_fl_A_ req_fl_A__eqMixin.
+
+    Definition req_fl_A := [eqType of req_fl_A_].
+
+  End req_fl_A__eq.
+
+  (* Concrete indications *)
   Inductive ind_fl_ : Type :=
   | Deliver_fl : node -> message -> ind_fl_.
 
   (* Equality *)
+  Section ind_fl__eq.
 
-  Definition eq_ind_fl_ (i i' : ind_fl_) : bool :=
-    match i, i' with
-    | Deliver_fl n m, Deliver_fl n' m' => [&& n == n' & m == m']
-    end.
+    Definition eq_ind_fl_ (r r' : ind_fl_) :=
+      match r, r' with
+      | Deliver_fl n m, Deliver_fl n' m' => (n == n') && (m == m')
+      end.
 
-  Lemma eq_ind_fl_P : Equality.axiom eq_ind_fl_.
-  Proof.
-    case => [ n m ];
-    case => [ n' m' ];
-    rewrite /=; try by constructor.
-    - (* Deliver_fl *)
-      case Hn: (n == n');
-        [move/eqP: Hn => ?; subst n' | constructor];
-        last by case=> ?; subst n'; rewrite eqxx in Hn.
-      case Hm: (m == m');
-        [move/eqP: Hm => ?; subst m' | constructor];
-        last by case=> ?; subst m'; rewrite eqxx in Hm.
-      by constructor.
-  Qed.
+    Lemma eq_ind_fl_P : Equality.axiom eq_ind_fl_.
+    Proof.
+      case=> [n m]; case=> [n' m'];
+        rewrite /eq_ind_fl_ /=; try by constructor.
+      - (* Deliver_fl *)
+        case Hn: (n == n');
+          [move/eqP: Hn => ?; subst n' | constructor];
+          last by case=> ?; subst n'; rewrite eqxx in Hn.
+        case Hm: (m == m');
+          [move/eqP: Hm => ?; subst m' | constructor];
+          last by case=> ?; subst m'; rewrite eqxx in Hm.
+        by constructor.
+    Qed.
 
-  Canonical ind_fl__eqMixin :=
-    Eval hnf in EqMixin eq_ind_fl_P.
-  Canonical ind_fl__eqType :=
-    Eval hnf in EqType ind_fl_ ind_fl__eqMixin.
+    Canonical ind_fl__eqMixin :=
+      Eval hnf in EqMixin eq_ind_fl_P.
+    Canonical ind_fl__eqType :=
+      Eval hnf in EqType ind_fl_ ind_fl__eqMixin.
 
-  Definition ind_fl := [eqType of ind_fl_].
+    Definition ind_fl := [eqType of ind_fl_].
+
+  End ind_fl__eq.
+
+  (* Assertion indications *)
+  Inductive ind_fl_A_ : Type :=
+  | Deliver_fl_A : node_variable -> message_variable -> ind_fl_A_.
+
+  (* Equality *)
+  Section ind_fl_A__eq.
+
+    Definition eq_ind_fl_A_ (r r' : ind_fl_A_) :=
+      match r, r' with
+      | Deliver_fl_A n m, Deliver_fl_A n' m' => (n == n') && (m == m')
+      end.
+
+    Lemma eq_ind_fl_A_P : Equality.axiom eq_ind_fl_A_.
+    Proof.
+      case=> [n m]; case=> [n' m'];
+        rewrite /eq_ind_fl_A_ /=; try by constructor.
+      - (* Deliver_fl_A *)
+        case Hn: (n == n');
+          [move/eqP: Hn => ?; subst n' | constructor];
+          last by case=> ?; subst n'; rewrite eqxx in Hn.
+        case Hm: (m == m');
+          [move/eqP: Hm => ?; subst m' | constructor];
+          last by case=> ?; subst m'; rewrite eqxx in Hm.
+        by constructor.
+    Qed.
+
+    Canonical ind_fl_A__eqMixin :=
+      Eval hnf in EqMixin eq_ind_fl_A_P.
+    Canonical ind_fl_A__eqType :=
+      Eval hnf in EqType ind_fl_A_ ind_fl_A__eqMixin.
+
+    Definition ind_fl_A := [eqType of ind_fl_A_].
+
+  End ind_fl_A__eq.
 
 End flc.
